Some further proof progress, and moving to Z3 4.8.5
Everest repo: branch z3-4.8.5 (04c80c8e)
fstarlang_binaries repo: branch z3-4.8.5 (19548b51)
FStar repo: branch z3-4.8.5 (cb7761cc)

Part of Hacl.Impl.QTesla.fst has "--admit_smt_queries true" but I don't
think it has anything to do with Z3; just still making my way through
updating my proofs.

qtesla/code/Hacl.Impl.QTesla.Constants.fst
@@ -3,11 +3,8 @@ module Hacl.Impl.QTesla.Constants
 open Lib.IntTypes
 open Hacl.SHA3
 
-//NS:
-//size is in terms of uint, which is abstract
-//normalize on constants is redundant
-let shake128_rate = size (normalize_term 168)
-let shake256_rate = size (normalize_term 136)
+unfold let shake128_rate = size 168
+unfold let shake256_rate = size 136
 
 // Implementation of cSHAKE gets inlined for extraction. To make things easier to compare to the
 // reference code, we enclose it in our own wrapper so it appears as a function call in callers.
