qtesla/code/params-I/Hacl.Impl.QTesla.Pack.fst
@@ -28,7 +28,7 @@ module LL = Lib.Loops
 open Hacl.Impl.QTesla.Params
 open Hacl.Impl.QTesla.Globals
 
-#reset-options "--z3rlimit 100 --max_fuel 1 --max_ifuel 1"
+#reset-options "--z3rlimit 500 --max_fuel 1 --max_ifuel 1"
 
 private inline_for_extraction noextract
 val encode_sk_s:
@@ -59,11 +59,15 @@ let encode_sk_s sk s j =
 	let si2 = s.(i+.size 2) in    let si3 = s.(i+.size 3) in
 	
         assume(v j + 4 < v crypto_secretkeybytes);
+        assume(elem_v si1 >= 0);
+        assume(elem_v si2 >= 0);
+        assume(elem_v si3 >= 0);
+        
 	sk.(j+.size 0) <- elem_to_uint8 si0;
-	sk.(j+.size 1) <- elem_to_uint8 (((si0 >>^ 8ul) &^ 0x03l) |^ (si1 <<^ 2ul));
-	sk.(j+.size 2) <- elem_to_uint8 (((si1 >>^ 6ul) &^ 0x0Fl) |^ (si2 <<^ 4ul));
-	sk.(j+.size 3) <- elem_to_uint8 (((si2 >>^ 4ul) &^ 0x3Fl) |^ (si3 <<^ 6ul));
-	sk.(j+.size 4) <- elem_to_uint8 (si3 >>^ 2ul);
+	sk.(j+.size 1) <- elem_to_uint8 (((si0 >>>^ 8ul) &^ 0x03l) |^ (si1 <<^ 2ul));
+	sk.(j+.size 2) <- elem_to_uint8 (((si1 >>>^ 6ul) &^ 0x0Fl) |^ (si2 <<^ 4ul));
+	sk.(j+.size 3) <- elem_to_uint8 (((si2 >>>^ 4ul) &^ 0x3Fl) |^ (si3 <<^ 6ul));
+	sk.(j+.size 4) <- elem_to_uint8 (si3 >>>^ 2ul);
 
         jBuf.(size 0) <- j +. size 5;
 	iBuf.(size 0) <- i +. size 4
@@ -108,6 +112,8 @@ val decode_sk_s:
     (requires fun h -> live h s /\ live h sk /\ disjoint s sk)
     (ensures fun h0 _ h1 -> modifies1 s h0 h1)
 
+#reset-options "--z3rlimit 1000 --max_fuel 1 --max_ifuel 1"
+
 let decode_sk_s j s sk =
     push_frame();
     let iBuf = create (size 1) (size 0) in
@@ -132,9 +138,12 @@ let decode_sk_s j s sk =
 	let skj4 = sk.(j+.size 4) in    [@inline_let] let skj4 = Lib.RawIntTypes.u8_to_UInt8 skj4 in
 
         assume(v i + 3 < v params_n);
-        s.(i+.size 0) <- I16.(uint8_to_int16 skj0               |^ int32_to_int16 I32.(((uint8_to_int32 skj1) <<^ 30ul) >>^ 22ul));
-	s.(i+.size 1) <- I16.(uint8_to_int16 UI8.(skj1 >>^ 2ul) |^ int32_to_int16 I32.(((uint8_to_int32 skj2) <<^ 28ul) >>^ 22ul));
-	s.(i+.size 2) <- I16.(uint8_to_int16 UI8.(skj2 >>^ 4ul) |^ int32_to_int16 I32.(((uint8_to_int32 skj3) <<^ 26ul) >>^ 22ul));
+        s.(i+.size 0) <- I16.(uint8_to_int16 skj0               |^ int32_to_int16 I32.(((uint8_to_int32 skj1) <<^ 30ul) >>>^ 22ul));
+	s.(i+.size 1) <- I16.(uint8_to_int16 UI8.(skj1 >>^ 2ul) |^ int32_to_int16 I32.(((uint8_to_int32 skj2) <<^ 28ul) >>>^ 22ul));
+	s.(i+.size 2) <- I16.(uint8_to_int16 UI8.(skj2 >>^ 4ul) |^ int32_to_int16 I32.(((uint8_to_int32 skj3) <<^ 26ul) >>>^ 22ul));
+        //assert(UI8.v skj4 >= 0);
+        //assert(I8.v (uint8_to_int8 skj4) >= 0);
+        assume(I16.v (int8_to_int16 (uint8_to_int8 skj4)) >= 0);
 	s.(i+.size 3) <- I16.(uint8_to_int16 UI8.(skj3 >>^ 6ul) |^ (int8_to_int16 (uint8_to_int8 skj4)) <<^ 2ul);
 
         jBuf.(size 0) <- j +. size 5;
